
ms: a owl:Ontology;
  rdfs:label "Multisensor Ontology";
  rdfs:comment "Defines various classes and properties used by the FP7 Multisensor project";
  rdfs:seeAlso <http://multisensorproject.eu>, <http://github.com/VladimirAlexiev/multisensor/>;
  dct:creator  <http://multisensorproject.eu>, <mailto:Vladimir.Alexiev@ontotext.com>;
  dct:created  "2016-06-20"^^xsd:date;
  dct:modified "2016-10-20"^^xsd:date;
  owl:versionInfo "1.0".

ms:GenericConcept a rdfs:Class;
  rdfs:subClassOf skos:Concept;
  rdfs:label "GenericConcept";
  rdfs:comment "Generic concept that doesn't belong to a specific domain";
  rdfs:isDefinedBy ms: .

ms:SpecificConcept a rdfs:Class;
  rdfs:subClassOf skos:Concept;
  rdfs:label "SpecificConcept";
  rdfs:comment "Concept that is specific to a Multisensor domain, determined by statistical analysis over the Multisensor SIMMO corpus";
  rdfs:isDefinedBy ms: .

ms:hasCaption a owl:ObjectProperty;
  rdfs:domain dctype:MovingImage;
  rdfs:range dctype:Text;
  rdfs:label "hasCaption";
  rdfs:comment "Transcript or ASR of a video (dctype:MovingImage) expressed as dctype:Text";
  rdfs:isDefinedBy ms: .

<http://data.multisensorproject.eu/agent/CAP> a prov:SoftwareAgent;
  foaf:name "Content Alignment Pipeline v1.0".

ms:linking-similar a owl:NamedIndividual, oa:Motivation;
  skos:inScheme oa:motivationScheme;
  skos:broader oa:linking;
  skos:prefLabel "linking-similar"@en;
  rdfs:comment "Motivation that represents a symmetric link between two *similar* articles"@en;
  rdfs:isDefinedBy ms: .

ms:linking-contradictory a owl:NamedIndividual, oa:Motivation;
  skos:inScheme oa:motivationScheme;
  skos:broader oa:linking;
  skos:prefLabel "linking-contradictory"@en;
  rdfs:comment "Motivation that represents a symmetric link between two *contradictory* articles"@en;
  rdfs:isDefinedBy ms: .

ms:score a owl:DatatypeProperty;
  rdfs:domain oa:Annotation;
  rdfs:range  xsd:decimal;
  rdfs:label "score"@en;
  rdfs:comment "Strength of an Annotation, eg the link between two entities"@en;
  rdfs:isDefinedBy ms: .

ms:has_page_rank a owl:DatatypeProperty;
  rdfs:domain sioc:Role;
  rdfs:label "Has page rank"@en;
  rdfs:comment "Centrality and importance of a poster on particular topic"@en;
  rdfs:isDefinedBy ms: .
 
ms:has_reachability a owl:DatatypeProperty;
  rdfs:domain sioc:Role;
  rdfs:label "Has reachability"@en;
  rdfs:comment "Level of linking of a poster on particular topic"@en;
  rdfs:isDefinedBy ms: .

ms:has_global_influence: a owl:DatatypeProperty;
  rdfs:domain sioc:Role;
  rdfs:label "Has global influence"@en;
  rdfs:comment "Global influence of a poster on particular topic. A combination of page rank and reachability"@en;
  rdfs:isDefinedBy ms: .

ms:negativePolarityValue a owl:DatatypeProperty;
  rdfs:domain marl:Opinion;
  rdfs:label "Most negative polarity value"@en;
  rdfs:comment "A sentence may include both negative and positive polarity words: this records the most negative polarity"@en;
  rdfs:isDefinedBy ms: .

ms:positivePolarityValue a owl:DatatypeProperty;
  rdfs:domain marl:Opinion;
  rdfs:label "Most positive polarity value"@en;
  rdfs:comment "A sentence may include both negative and positive polarity words: this records the most positive polarity"@en;
  rdfs:isDefinedBy ms: .

ms:sentimentalityValue a owl:DatatypeProperty;
  rdfs:domain marl:Opinion;
  rdfs:label "Sentimentality value"@en;
  rdfs:comment """How strong is the sentiment.
Sum of the absolute values of the most positive and most negative polarity of an opinion (i.e. the difference between them)"""@en;
  rdfs:isDefinedBy ms: .

ms:fluency a owl:DatatypeProperty;
  rdfs:domain nif:Context;
  rdfs:label "Text fluency"@en;
  rdfs:comment """How fluent is the text.
The text should build from sentence to sentence to a coherent body of information about a topic. 
Consecutive sentences should be meaningfully connected. Paragraphs should be written in a logical sequence. 
The best way to achieve fluency is to have at least one object or subject repeatedly mentioned in consecutive units of text. """@en;
  rdfs:comment "Range: 1.0 ... 5.0"@en;
  rdfs:isDefinedBy ms: .

ms:richness a owl:DatatypeProperty;
  rdfs:domain nif:Context;
  rdfs:label "Text richness"@en;
  rdfs:comment """How rich is the text. 
Is the writing style and vocabulary used rich and interesting, as opposed to plain and straightforward?"""@en;
  rdfs:comment "Range: 1.0 ... 5.0"@en;
  rdfs:isDefinedBy ms: .

ms:technicality a owl:DatatypeProperty;
  rdfs:domain nif:Context;
  rdfs:label "Text technicality"@en;
  rdfs:comment """How technical is the text. 
Are the topic and used language technical? 
Does it require effort and previous knowledge to understand the text?"""@en;
  rdfs:comment "Range: 1.0 ... 5.0"@en;
  rdfs:isDefinedBy ms: .
